src/BS.v
@@ -2,13 +2,12 @@
    BS stands for "Binary String".  May be instantiated with 
    types like strings and byte buffers in concrete implementations.    *)
 
-Require Import String. 
+Require Import StringT ResultT. 
 
-Definition BS : Set.
-Admitted.
+Definition BS : Set. Admitted.
 
-Definition BS_to_string (bs:BS) : string. Admitted.
-Definition string_to_BS (s:string) : option BS. Admitted.
+Definition BS_to_stringT (bs:BS) : StringT. Admitted.
+Definition stringT_to_BS (s: StringT) : ResultT BS StringT. Admitted.
 
 (* Some default/reserved BS values *)
 Definition default_bs : BS. Admitted.
