src/Example_Phrases_Demo_Admits.v
@@ -13,31 +13,31 @@ Definition dest_plc : Plc. Admitted.
 
 Definition cal_ak_targid : ASP_ID. Admitted.
 Definition cal_ak_aspid : ASP_ID. Admitted.
-Definition cal_ak_args : list Arg. Admitted.
+Definition cal_ak_args : ASP_ARGS. Admitted.
 
 Definition pub_bc_targid : ASP_ID. Admitted.
 Definition pub_bc_aspid : ASP_ID. Admitted.
-Definition pub_bc_args : list Arg. Admitted.
+Definition pub_bc_args : ASP_ARGS. Admitted.
 
 Definition get_data_targid : ASP_ID. Admitted.
 Definition get_data_aspid : ASP_ID. Admitted.
-Definition get_data_args : list Arg. Admitted.
+Definition get_data_args : ASP_ARGS. Admitted.
 
 Definition tpm_sig_targid : ASP_ID. Admitted.
 Definition tpm_sig_aspid : ASP_ID. Admitted.
-Definition tpm_sig_args : list Arg. Admitted.
+Definition tpm_sig_args : ASP_ARGS. Admitted.
 
 Definition ssl_enc_targid : ASP_ID. Admitted.
 Definition ssl_enc_aspid : ASP_ID. Admitted.
-Definition ssl_enc_args : list Arg. Admitted.
+Definition ssl_enc_args : ASP_ARGS. Admitted.
 
 Definition store_clientData_targid : ASP_ID. Admitted.
 Definition store_clientData_aspid : ASP_ID. Admitted.
-Definition store_clientData_args : list Arg. Admitted.
+Definition store_clientData_args : ASP_ARGS. Admitted.
 
 Definition ssl_sig_targid : ASP_ID. Admitted.
 (* Definition ssl_sig_aspid : ASP_ID. Admitted. *)
-Definition ssl_sig_args : list Arg. Admitted.
+Definition ssl_sig_args : ASP_ARGS. Admitted.
 
 
 Definition demo_plc_1 : ID_Type. Admitted.
@@ -45,8 +45,8 @@ Definition demo_plc_2 : ID_Type. Admitted.
 
 Definition kim_meas_targid : ASP_ID. Admitted.
 Definition kim_meas_aspid : ASP_ID. Admitted.
-Definition kim_meas_args : list Arg. Admitted.
+Definition kim_meas_args : ASP_ARGS. Admitted.
 
 Definition cm_targid : ASP_ID. Admitted.
 Definition cm_aspid : ASP_ID. Admitted.
-Definition cm_args : list Arg. Admitted.
+Definition cm_args : ASP_ARGS. Admitted.
