src/Interface_Strings_Admits.v
@@ -16,3 +16,10 @@ Definition STR_NEGOTIATE : StringT. Admitted.
 Definition STR_APPRAISE : StringT. Admitted.
 Definition STR_REQUEST : StringT. Admitted.
 Definition STR_RESPONSE : StringT. Admitted.
+
+(* ASP String Admits *)
+Definition STR_ASP_RUN : StringT. Admitted.
+Definition STR_ASP_ID : StringT. Admitted.
+Definition STR_ASP_ARGS : StringT. Admitted.
+Definition STR_TARG_PLC : StringT. Admitted.
+Definition STR_TARG : StringT. Admitted.
