src/Manifest_Compiler.v
@@ -2,140 +2,134 @@
     Takes a Manifest + AM_Library to an AM_Config.  *)
 
 Require Import Maps AbstractedTypes EqClass Term_Defs_Core Manifest_Admits Manifest
-  ErrorStMonad_Coq Term_Defs.
-
-Require Import Manifest_Set.
-  
+  ErrorStMonad_Coq Term_Defs Interface_Types CvmJson_Interfaces Manifest_Set
+  IO_Stubs.
 
 Require Import List.
 Import ListNotations.
   
-  (* Reduces a MapC to only include elements that satisfy the condition "f" *)
-  Fixpoint minify_mapC {A B : Type} `{HA : EqClass A} (m : MapC A B) (f : A -> bool) : (MapC A B) :=
-    match m with
-    | nil => nil
-    | cons (k,v) tl => if (f k) then cons (k,v) (minify_mapC tl f) else minify_mapC tl f
+(* Reduces a MapC to only include elements that satisfy the condition "f" *)
+Fixpoint minify_mapC {A B : Type} `{HA : EqClass A} (m : MapC A B) (f : A -> bool) : (MapC A B) :=
+  match m with
+  | nil => nil
+  | cons (k,v) tl => if (f k) then cons (k,v) (minify_mapC tl f) else minify_mapC tl f
+  end.
+
+(* Reduces a MapD to only include elements that satisfy the condition "f" *)
+Fixpoint minify_mapD {A B : Type} `{HA : EqClass A} `{HB : EqClass B} (m : MapD A B) (f : A -> bool) : (MapD A B) :=
+  match m with
+  | nil => nil
+  | cons (k,v) tl => if (f k) then cons (k,v) (minify_mapD tl f) else minify_mapD tl f
+  end.
+
+Definition generate_ASP_dispatcher' (al : AM_Library) (am : Manifest) (par : ASP_PARAMS) (rawEv : RawEv) : ResultT RawEv DispatcherErrors :=
+  let (aspid, args, targ_plc, targ) := par in
+  let abstract_asps := am.(asps) in
+  let local_asps_map := al.(Lib_ASPS) in
+  let shrunk_map : (MapC ASP_ID ASP_Locator) := 
+  minify_mapC local_asps_map (fun x => if (in_dec_set x abstract_asps) then true else false) 
+  in
+    (* check is the ASPID is available *) 
+    match (map_get shrunk_map aspid) with
+    | Some loc => 
+      let asp_req := (mkASPRReq aspid args targ_plc targ rawEv) in
+      let js_req := ASPRunRequest_to_JSON asp_req in
+      (* Used to tell difference between local and remote ASPs *)
+      let js_resp := (match loc with
+                      | Local_ASP fsLoc => make_JSON_FS_Location_Request fsLoc js_req
+                      | Remote_ASP uuid => make_JSON_Network_Request uuid js_req
+                      end) in
+      match JSON_to_ASPRunResponse js_resp with
+      | resultC r => 
+          let '(mkASPRResp succ ev) := r in
+          resultC ev
+      | errC msg => errC (Runtime msg)
+      end
+    | None => errC Unavailable
     end.
 
-  (* Reduces a MapD to only include elements that satisfy the condition "f" *)
-  Fixpoint minify_mapD {A B : Type} `{HA : EqClass A} `{HB : EqClass B} (m : MapD A B) (f : A -> bool) : (MapD A B) :=
-    match m with
-    | nil => nil
-    | cons (k,v) tl => if (f k) then cons (k,v) (minify_mapD tl f) else minify_mapD tl f
+(* This function will be a dispatcher for either local ASPS to CakeMLCallback, or pass them off to the ASP_Server *)
+Definition generate_ASP_dispatcher `{HID : EqClass ID_Type} (al : AM_Library) (am : Manifest)
+    : (ASPCallback DispatcherErrors) :=
+  (* let asp_server_cb := al.(ASPServer_Cb) in *)
+    (generate_ASP_dispatcher' al am). 
+
+Definition generate_appraisal_ASP_dispatcher' (al : AM_Library) (am : Manifest) (par : ASP_PARAMS) (rawEv : RawEv) :=
+  let (aspid, args, targ_plc, targ) := par in
+  let abstract_asps := am.(appraisal_asps) in
+  let local_asps_map := al.(Lib_Appraisal_ASPS) in
+  let shrunk_map : (MapC (Plc*ASP_ID) ASP_Locator) :=  
+  minify_mapC local_asps_map (fun x => if (in_dec_set x abstract_asps) then true else false) in
+    (* check is the ASPID is a local, with a callback *)
+    match (map_get shrunk_map (targ_plc,aspid)) with
+    | Some loc => 
+      let asp_req := (mkASPRReq aspid args targ_plc targ rawEv) in
+      let js_req := ASPRunRequest_to_JSON asp_req in
+      (* Used to tell difference between local and remote ASPs *)
+      let js_resp := (match loc with
+                      | Local_ASP fsLoc => make_JSON_FS_Location_Request fsLoc js_req
+                      | Remote_ASP uuid => make_JSON_Network_Request uuid js_req
+                      end) in
+      match JSON_to_ASPRunResponse js_resp with
+      | resultC r => 
+          let '(mkASPRResp succ ev) := r in
+          resultC ev
+      | errC msg => errC (Runtime msg)
+      end
+    | None => errC Unavailable
     end.
 
-  Definition generate_ASP_dispatcher' (al : AM_Library) (am : Manifest) (par : ASP_PARAMS) (p : Plc) (bs : BS) (rawEv : RawEv) :=
-        let (aspid, args, plc, targ) := par in
-        let abstract_asps := am.(asps) in
-        let local_asps_map := al.(Local_ASPS) in
-        let shrunk_map : (MapC ASP_ID (ASPCallback CallBackErrors)) := 
-        minify_mapC local_asps_map (fun x => if (in_dec_set x abstract_asps) then true else false) in
-          (* check is the ASPID is a local, with a callback *)
-          match (map_get shrunk_map aspid) with
-          | Some cb => 
-            match (cb par p bs rawEv) with
-            | resultC r => resultC r
-            | errC (messageLift msg) => 
-                errC (Runtime msg)
-            end
-          | None => errC Unavailable 
-            (* (asp_server_cb asp_server_addr par) *)
-          end.
 
-  (* This function will be a dispatcher for either local ASPS to CakeMLCallback, or pass them off to the ASP_Server *)
-  Definition generate_ASP_dispatcher `{HID : EqClass ID_Type} (al : AM_Library) (am : Manifest)
-      : (ASPCallback DispatcherErrors) :=
-    (* let asp_server_cb := al.(ASPServer_Cb) in *)
-      (generate_ASP_dispatcher' al am). 
+Definition generate_appraisal_ASP_dispatcher `{HID : EqClass ID_Type} (al : AM_Library) (am : Manifest)
+: (ASPCallback DispatcherErrors) :=
+(* let asp_server_cb := al.(ASPServer_Cb) in *)
+(generate_appraisal_ASP_dispatcher' al am). 
 
 
+(* This function will lookup for either local Plcs to UUID, or pass them off to the Plc Server *)
+Definition generate_Plc_dispatcher `{HID : EqClass ID_Type} (al : AM_Library) (am : Manifest) 
+    : PlcCallback :=
+  (* let plc_server_cb := al.(PlcServer_Cb) in *)
+    let local_plc_map := al.(Lib_Plcs) in
+    let abstract_plcs := am.(uuidPlcs) in
+    let shrunk_map := 
+      minify_mapD local_plc_map (fun x => if (in_dec_set x abstract_plcs) then true else false) in
 
-  Definition generate_appraisal_ASP_dispatcher' (al : AM_Library) (am : Manifest) (par : ASP_PARAMS) (p : Plc) (bs : BS) (rawEv : RawEv) :=
-    let (aspid, args, plc, targ) := par in
-    let abstract_asps := am.(appraisal_asps) in
-    let local_asps_map := al.(Local_Appraisal_ASPS) in
-    let shrunk_map : (MapC (Plc*ASP_ID) (ASPCallback CallBackErrors)) :=  
-    minify_mapC local_asps_map (fun x => if (in_dec_set x abstract_asps) then true else false) in
-      (* check is the ASPID is a local, with a callback *)
-      match (map_get shrunk_map (p,aspid)) with
-      | Some cb => 
-        match (cb par p bs rawEv) with
-        | resultC r => resultC r
-        | errC (messageLift msg) => 
-            errC (Runtime msg)
-        end
-      | None => errC Unavailable 
-        (* (asp_server_cb asp_server_addr par) *)
+    fun (p : Plc) =>
+      (* check is the plc "p" is local, with a reference *)
+      match (map_get shrunk_map p) with
+      | Some uuid => resultC uuid
+      | None => errC Unavailable
+        (* (plc_server_cb plc_server_addr p) *)
+      end.
+    
+(* This function will lookup the PubKey either locally Plc -> PublicKey or pass off to PubKeyServer *)
+Definition generate_PubKey_dispatcher `{HID : EqClass ID_Type} (al : AM_Library) (am : Manifest) 
+    : PubKeyCallback :=
+  (* let pubkey_server_cb := al.(PubKeyServer_Cb) in *)
+    let local_pubkey_map := al.(Lib_PubKeys) in
+    let abstract_plcs := am.(pubKeyPlcs) in
+    let shrunk_map := 
+      minify_mapD local_pubkey_map (fun x => if (in_dec_set x abstract_plcs) then true else false) in
+
+    fun (p : Plc) =>
+      (* check is the plc "p" is local, with a reference in the pubkey server mapping *)
+      match (map_get shrunk_map p) with
+      | Some key => resultC key
+      | None => errC Unavailable
+        (* (pubkey_server_cb pubkey_server_addr p) *)
       end.
 
-
-  Definition generate_appraisal_ASP_dispatcher `{HID : EqClass ID_Type} (al : AM_Library) (am : Manifest)
-  : (ASPCallback DispatcherErrors) :=
-(* let asp_server_cb := al.(ASPServer_Cb) in *)
-  (generate_appraisal_ASP_dispatcher' al am). 
-
-
-  (* This function will lookup for either local Plcs to UUID, or pass them off to the Plc Server *)
-  Definition generate_Plc_dispatcher `{HID : EqClass ID_Type} (al : AM_Library) (am : Manifest) 
-      : PlcCallback :=
-    (* let plc_server_cb := al.(PlcServer_Cb) in *)
-      let local_plc_map := al.(Local_Plcs) in
-      let abstract_plcs := am.(uuidPlcs) in
-      let shrunk_map := 
-        minify_mapD local_plc_map (fun x => if (in_dec_set x abstract_plcs) then true else false) in
-
-      fun (p : Plc) =>
-        (* check is the plc "p" is local, with a reference *)
-        match (map_get shrunk_map p) with
-        | Some uuid => resultC uuid
-        | None => errC Unavailable
-          (* (plc_server_cb plc_server_addr p) *)
-        end.
-      
-  (* This function will lookup the PubKey either locally Plc -> PublicKey or pass off to PubKeyServer *)
-  Definition generate_PubKey_dispatcher `{HID : EqClass ID_Type} (al : AM_Library) (am : Manifest) 
-      : PubKeyCallback :=
-    (* let pubkey_server_cb := al.(PubKeyServer_Cb) in *)
-      let local_pubkey_map := al.(Local_PubKeys) in
-      let abstract_plcs := am.(pubKeyPlcs) in
-      let shrunk_map := 
-        minify_mapD local_pubkey_map (fun x => if (in_dec_set x abstract_plcs) then true else false) in
-
-      fun (p : Plc) =>
-        (* check is the plc "p" is local, with a reference in the pubkey server mapping *)
-        match (map_get shrunk_map p) with
-        | Some key => resultC key
-        | None => errC Unavailable
-          (* (pubkey_server_cb pubkey_server_addr p) *)
-        end.
-
-  Definition generate_UUID_dispatcher `{HID : EqClass ID_Type} (al : AM_Library) (am : Manifest)  
-      : UUIDCallback :=
-    (* let uuid_server_cb := al.(UUIDServer_Cb) in *)
-      let local_plc_map := al.(Local_Plcs) in
-      let abstract_plcs := am.(uuidPlcs) in
-      let shrunk_map :=
-        minify_mapD local_plc_map (fun x => if (in_dec_set x abstract_plcs) then true else false) in
-
-      fun (u : UUID) =>
-        (* check if uuid "u" is local, else dispatch to callback *)
-        match (mapD_get_key shrunk_map u) with
-        | Some p => resultC p
-        | None => errC Unavailable
-          (* (uuid_server_cb local_uuid_addr u) *)
-        end.
-
-  (* This is a rough type signature for the "manifest compiler".  Still some details to be ironed out... *)
-  Definition manifest_compiler (m : Manifest) (al : AM_Library) : AM_Config :=
-  (* The output of this function is an AM Config, and a 
-  function that can be used like "check_asp_EXTD".
-  This function will be used in extraction to either dispatch ASPs to the ASP server, or call a local callback *)
-  {|
-    absMan   := m ;
-    am_clone_addr := (UUID_AM_Clone al) ;
-    aspCb     := (generate_ASP_dispatcher al m) ;
-    app_aspCb := (generate_appraisal_ASP_dispatcher al m);
-    plcCb     := (generate_Plc_dispatcher al m);
-    pubKeyCb  := (generate_PubKey_dispatcher al m);
-    uuidCb    := (generate_UUID_dispatcher al m);
-  |}.
+(* This is a rough type signature for the "manifest compiler".  Still some details to be ironed out... *)
+Definition manifest_compiler (m : Manifest) (al : AM_Library) : AM_Config :=
+(* The output of this function is an AM Config, and a 
+function that can be used like "check_asp_EXTD".
+This function will be used in extraction to either dispatch ASPs to the ASP server, or call a local callback *)
+{|
+  absMan   := m ;
+  am_clone_addr := (UUID_AM_Clone al) ;
+  aspCb     := (generate_ASP_dispatcher al m) ;
+  app_aspCb := (generate_appraisal_ASP_dispatcher al m);
+  plcCb     := (generate_Plc_dispatcher al m);
+  pubKeyCb  := (generate_PubKey_dispatcher al m);
+|}.
